TryInc updates

Test/civl/samples/TryIncNBelowMax.bpl
@@ -4,7 +4,7 @@
 var {:layer 0, 2} count: int;
 const max: int;
 
-yield procedure {:layer 1} TryIncBelowMax() returns (ok: bool)
+yield procedure {:layer 1} TryIncBelowNMax() returns (ok: bool)
 requires call Yield1();
 refines atomic action {:layer 2} _ {
     if (ok) {
@@ -13,14 +13,14 @@ refines atomic action {:layer 2} _ {
     }
 }
 {
-    var retry_limit: int;
+    var limit: int;
 
-    call retry_limit := ComputeLimit() | Yield1();
+    call limit := ComputeLimit() | Yield1();
     async call backgroundMaintenance();
-    call ok := HelperInc(0, retry_limit);
+    call ok := HelperInc(1, limit);
 }
 
-yield procedure {:layer 1} HelperInc(tries: int, retry_limit: int) returns (ok: bool)
+yield procedure {:layer 1} HelperInc(tries: int, limit: int) returns (ok: bool)
 requires call Yield1();
 refines atomic action {:layer 2} _ {
     if (ok) {
@@ -31,12 +31,10 @@ refines atomic action {:layer 2} _ {
 {
     var n: int;
 
-    if (tries > retry_limit) {
+    if (tries >= limit) {
         ok := false; // retry limit reached
         return; 
     }
-
-    call Yield1();
 
     call n := Read();
     if (n >= max) {
@@ -50,33 +48,31 @@ refines atomic action {:layer 2} _ {
     if (ok) {
         return;
     }
-    call ok := HelperInc(tries+1, retry_limit);
+    call ok := HelperInc(tries+1, limit);
 }
 
-yield procedure {:layer 1} ComputeLimit() returns (retry_limit: int)
+yield procedure {:layer 1} ComputeLimit() returns (limit: int)
 refines atomic action {:layer 2} _ {
-    assume retry_limit > 0;
+    assume limit > 0;
 }
 {
-    assume retry_limit > 0;
+    assume limit > 0;
 }
 
 
 yield procedure {:layer 1} backgroundMaintenance() 
-preserves call Yield1();
+requires call Yield1();
 {
     assert {:layer 1} count <= max; 
 }
 
-yield procedure {:layer 0} CAS(prev: int, next: int) returns (status: bool);
+yield procedure {:layer 0} CAS(prev: int, next: int) returns (ok: bool);
 refines atomic action {:layer 1} _ {
     assert prev < max; 
-    status := (count == prev); 
-
-    if (status) {
+   ok := (count == prev);
+    if (ok) {
         count := next;
-        status := true;
-    } 
+    }
 }
 
 yield procedure {:layer 0} Read() returns (val: int);
